simulation proof with other changes

ds_abs1/ds_abs1_rxScript.sml
@@ -9,28 +9,27 @@ val SPI_ABS1_RX_ENABLE_def = Define `
 SPI_ABS1_RX_ENABLE (ds_abs1:ds_abs1_state) =
 ((ds_abs1.state = abs1_rx_idle) \/
 (ds_abs1.state = abs1_rx_update) \/
-(ds_abs1.state = abs1_rx_next) \/
-(ds_abs1.state = abs1_rx_stop))`
+(ds_abs1.state = abs1_rx_next))`
 
 (* DRIVER_ABS1_RX_ENABLE: ds_abs1_state -> bool *)
 val DRIVER_ABS1_RX_ENABLE_def = Define `
 DRIVER_ABS1_RX_ENABLE (ds_abs1:ds_abs1_state) =
-((ds_abs1.state = abs1_rx_fetch_data) \/
+((ds_abs1.state = abs1_rx_ready) \/
+(ds_abs1.state = abs1_rx_fetch_data) \/
 (ds_abs1.state = abs1_rx_next) \/
 (ds_abs1.state = abs1_rx_next_ready))`
 
 (* COMB_ABS1_RX_ENABLE: ds_abs1_state -> bool *)
 val COMB_ABS1_RX_ENABLE_def = Define `
 COMB_ABS1_RX_ENABLE (ds_abs1:ds_abs1_state) =
-((ds_abs1.state = abs1_rx_ready) \/
+((ds_abs1.state = abs1_rx_read) \/
 (ds_abs1.state = abs1_rx_reset))`
 
 (* ABS1_RX_LBL_ENABLE: ds_abs1_state -> bool *)
 val ABS1_RX_LBL_ENABLE_def = Define `
 ABS1_RX_LBL_ENABLE (ds_abs1:ds_abs1_state) =
 ((ds_abs1.state = abs1_rx_receive) \/
-(ds_abs1.state = abs1_rx_fetch_data) \/
-(ds_abs1.state = abs1_rx_done))`
+(ds_abs1.state = abs1_rx_fetch_data))`
 
 (* tau_spi related functions *)
 (* spi_abs1_rx_idle_op: ds_abs1_state -> ds_abs1_state *)
@@ -48,11 +47,6 @@ val spi_abs1_rx_next_op_def = Define `
 spi_abs1_rx_next_op (ds_abs1:ds_abs1_state) =
 ds_abs1 with state := abs1_rx_next_ready`
 
-(* spi_abs1_rx_stop_op: ds_abs1_state -> ds_abs1_state *)
-val spi_abs1_rx_stop_op_def = Define `
-spi_abs1_rx_stop_op (ds_abs1:ds_abs1_state) =
-ds_abs1 with state := abs1_rx_reset`
-
 (* spi_abs_rx_operations: ds_abs1_state -> ds_abs1_state *)
 val spi_abs1_rx_operations_def = Define `
 spi_abs1_rx_operations (ds_abs1:ds_abs1_state) =
@@ -62,19 +56,23 @@ else if (ds_abs1.state = abs1_rx_update) then
 (spi_abs1_rx_update_op ds_abs1)
 else if (ds_abs1.state = abs1_rx_next) then
 (spi_abs1_rx_next_op ds_abs1)
-else if (ds_abs1.state = abs1_rx_stop) then
-(spi_abs1_rx_stop_op ds_abs1)
 else ds_abs1 with err := T`
 
 
 (* tau_dr related functions *)
+(* driver_abs1_rx_ready_op: ds_abs1_state -> ds_abs1_state *)
+val driver_abs1_rx_ready_op_def = Define `
+driver_abs1_rx_ready_op (ds_abs1:ds_abs1_state) =
+ds_abs1 with 
+state := if ds_abs1.ds_abs1_rx.rx_left_length > 0 then abs1_rx_read else abs1_rx_reset`
+
 (* driver_abs1_rx_fetch_data_op: ds_abs1_state -> ds_abs1_state *)
 val driver_abs1_rx_fetch_data_op_def = Define `
 driver_abs1_rx_fetch_data_op (ds_abs1:ds_abs1_state) =
 ds_abs1 with <| ds_abs1_rx := ds_abs1.ds_abs1_rx with
 <| rx_data_buffer := ds_abs1.ds_abs1_rx.rx_data_buffer ++ [ds_abs1.spi_abs1.RX_SHIFT_REG]; 
    rx_left_length := ds_abs1.ds_abs1_rx.rx_left_length - 1 |>;
-state := if ds_abs1.ds_abs1_rx.rx_left_length > 1 then abs1_rx_receive else abs1_rx_done |>`
+state := abs1_rx_receive |>`
 
 (* driver_abs1_rx_next_op: ds_abs1_state -> ds_abs1_state *)
 val driver_abs1_rx_next_op_def = Define `
@@ -82,7 +80,7 @@ driver_abs1_rx_next_op (ds_abs1:ds_abs1_state) =
 ds_abs1 with <| ds_abs1_rx := ds_abs1.ds_abs1_rx with
 <| rx_data_buffer := ds_abs1.ds_abs1_rx.rx_data_buffer ++ [ds_abs1.ds_abs1_rx.temp_value];
    rx_left_length := ds_abs1.ds_abs1_rx.rx_left_length - 1 |>;
-state := if ds_abs1.ds_abs1_rx.rx_left_length > 1 then abs1_rx_update else abs1_rx_stop |>`
+state := abs1_rx_update |>`
 
 (* driver_abs1_rx_next_ready_op: ds_abs1_state -> ds_abs1_state *)
 val driver_abs1_rx_next_ready_op_def = Define `
@@ -90,12 +88,14 @@ driver_abs1_rx_next_ready_op (ds_abs1: ds_abs1_state) =
 ds_abs1 with <| ds_abs1_rx := ds_abs1.ds_abs1_rx with 
 <| rx_data_buffer := ds_abs1.ds_abs1_rx.rx_data_buffer ++ [ds_abs1.ds_abs1_rx.temp_value];
    rx_left_length := ds_abs1.ds_abs1_rx.rx_left_length - 1 |>;
-state := if ds_abs1.ds_abs1_rx.rx_left_length > 1 then abs1_rx_ready else abs1_rx_reset |>`
+state := abs1_rx_ready |>`
 
 (* driver_abs1_rx_operations: ds_abs1_state -> ds_abs1_state *)
 val driver_abs1_rx_operations_def = Define `
 driver_abs1_rx_operations (ds_abs1:ds_abs1_state) =
-if (ds_abs1.state = abs1_rx_fetch_data) then
+if (ds_abs1.state = abs1_rx_ready) then
+(driver_abs1_rx_ready_op ds_abs1)
+else if (ds_abs1.state = abs1_rx_fetch_data) then
 (driver_abs1_rx_fetch_data_op ds_abs1)
 else if (ds_abs1.state = abs1_rx_next) then
 (driver_abs1_rx_next_op ds_abs1)
@@ -105,9 +105,9 @@ else ds_abs1 with err:= T`
 
 
 (* tau_comb related functions *)
-(* comb_abs1_rx_ready_op: ds_abs1_state -> ds_abs1_state *)
-val comb_abs1_rx_ready_op_def = Define `
-comb_abs1_rx_ready_op (ds_abs1:ds_abs1_state) =
+(* comb_abs1_rx_read_op: ds_abs1_state -> ds_abs1_state *)
+val comb_abs1_rx_read_op_def = Define `
+comb_abs1_rx_read_op (ds_abs1:ds_abs1_state) =
 ds_abs1 with <| state := abs1_rx_fetch_data;
 ds_abs1_rx := ds_abs1.ds_abs1_rx with temp_value := ds_abs1.spi_abs1.RX_SHIFT_REG |>`
 
@@ -119,8 +119,8 @@ ds_abs1 with state := abs1_ready`
 (* comb_abs1_rx_operations: ds_abs1_state -> ds_abs1_state *)
 val comb_abs1_rx_operations_def = Define `
 comb_abs1_rx_operations (ds_abs1:ds_abs1_state) =
-if ds_abs1.state = abs1_rx_ready 
-then (comb_abs1_rx_ready_op ds_abs1)
+if ds_abs1.state = abs1_rx_read 
+then (comb_abs1_rx_read_op ds_abs1)
 else if ds_abs1.state = abs1_rx_reset
 then (comb_abs1_rx_reset_op ds_abs1)
 else ds_abs1 with err := T`
@@ -147,16 +147,7 @@ val abs1_rx_fetch_data_op_def = Define `
 abs1_rx_fetch_data_op (ds_abs1:ds_abs1_state) (data:word8 option) =
 ds_abs1 with 
 <| state := abs1_rx_next;
-   spi_abs1 := ds_abs1.spi_abs1 with RX_SHIFT_REG := THE data;
-   (*ds_abs1_rx := ds_abs1.ds_abs1_rx with temp_value := ds_abs1.spi_abs1.RX_SHIFT_REG*) |>`
-
-(* abs1_rx_done_op: ds_abs1_state -> word8 option -> ds_abs1_state *)
-val abs1_rx_done_op_def = Define `
-abs1_rx_done_op (ds_abs1:ds_abs1_state) (data:word8 option) =
-ds_abs1 with 
-<| state := abs1_rx_stop;
    spi_abs1 := ds_abs1.spi_abs1 with RX_SHIFT_REG := THE data |>`
-
 
 (* abs1_rx_receive_data_op: ds_abs1_state -> word8 option -> ds_abs1_state *)
 val abs1_rx_receive_data_op_def = Define `
@@ -165,8 +156,6 @@ if (ds_abs1.state = abs1_rx_receive) then
 (abs1_rx_receive_op ds_abs1 data)
 else if (ds_abs1.state = abs1_rx_fetch_data) then 
 (abs1_rx_fetch_data_op ds_abs1 data)
-else if (ds_abs1.state = abs1_rx_done) then 
-(abs1_rx_done_op ds_abs1 data)
 else ds_abs1 with err := T`
 
 val _ = export_theory();
