ds_abs1/ds_abs1_txScript.sml
@@ -9,12 +9,15 @@ val SPI_ABS1_TX_ENABLE_def = Define `
 SPI_ABS1_TX_ENABLE (ds_abs1:ds_abs1_state) =
 ((ds_abs1.state = abs1_tx_idle) \/ 
 (ds_abs1.state = abs1_tx_data_1) \/
-(ds_abs1.state = abs1_tx_data_2))`
+(ds_abs1.state = abs1_tx_data_2) \/
+(ds_abs1.state = abs1_tx_update) \/
+(ds_abs1.state = abs1_tx_last_update))`
 
 (* COMB_ABS1_TX_ENABLE: ds_abs1_state -> bool *)
 val COMB_ABS1_TX_ENABLE_def = Define `
 COMB_ABS1_TX_ENABLE (ds_abs1:ds_abs1_state) =
 ((ds_abs1.state = abs1_tx_trans) \/
+(ds_abs1.state = abs1_tx_done_2) \/
 (ds_abs1.state = abs1_tx_reset))`
 
 (* tau_spi related functions *)
@@ -39,6 +42,22 @@ spi_abs1 := ds_abs1.spi_abs1 with
 TX_SHIFT_REG := (EL (ds_abs1.ds_abs1_tx.tx_cur_length - 1) 
 (ds_abs1.ds_abs1_tx.tx_data_buffer)) |>`
 
+(* spi_abs1_tx_update_op: ds_abs1_state -> ds_abs1_state *)
+val spi_abs1_tx_update_op_def = Define `
+spi_abs1_tx_update_op (ds_abs1:ds_abs1_state) =
+ds_abs1 with <| state := abs1_tx_done_2;
+spi_abs1 := ds_abs1.spi_abs1 with
+TX_SHIFT_REG := (EL (ds_abs1.ds_abs1_tx.tx_cur_length - 1)
+(ds_abs1.ds_abs1_tx.tx_data_buffer)) |>`
+
+(* spi_abs1_tx_last_update_op: ds_abs1_state -> ds_abs1_state *)
+val spi_abs1_tx_last_update_op_def = Define `
+spi_abs1_tx_last_update_op (ds_abs1:ds_abs1_state) =
+ds_abs1 with <| state := abs1_tx_done_1;
+spi_abs1 := ds_abs1.spi_abs1 with
+TX_SHIFT_REG := (EL (ds_abs1.ds_abs1_tx.tx_cur_length - 1) 
+(ds_abs1.ds_abs1_tx.tx_data_buffer)) |>`
+
 (* spi_abs1_tx_operations: ds_abs1_state -> ds_abs1_state *)
 val spi_abs1_tx_operations_def = Define `
 spi_abs1_tx_operations (ds_abs1:ds_abs1_state) =
@@ -48,16 +67,28 @@ else if (ds_abs1.state = abs1_tx_data_1) then
 (spi_abs1_tx_data_1_op ds_abs1)
 else if (ds_abs1.state = abs1_tx_data_2) then
 (spi_abs1_tx_data_2_op ds_abs1)
+else if (ds_abs1.state = abs1_tx_update) then
+(spi_abs1_tx_update_op ds_abs1)
+else if (ds_abs1.state = abs1_tx_last_update) then
+(spi_abs1_tx_last_update_op ds_abs1)
 else ds_abs1 with err := T`
 
 
 (* tau_comb related functions *)
-(* comb_abs1_tx_trans_op ds_abs1_state -> ds_abs1_state *)
+(* comb_abs1_tx_trans_op: ds_abs1_state -> ds_abs1_state *)
 val comb_abs1_tx_trans_op_def = Define `
 comb_abs1_tx_trans_op (ds_abs1:ds_abs1_state) =
 ds_abs1 with <| 
 state := if ds_abs1.ds_abs1_tx.tx_cur_length < ((LENGTH ds_abs1.ds_abs1_tx.tx_data_buffer) - 1)
 then abs1_tx_data_2 else abs1_tx_data_1;
+ds_abs1_tx := ds_abs1.ds_abs1_tx with tx_cur_length := ds_abs1.ds_abs1_tx.tx_cur_length + 1 |>`
+
+(* comb_abs1_tx_done_2_op: ds_abs1_state -> ds_abs1_state *)
+val comb_abs1_tx_done_2_op_def = Define `
+comb_abs1_tx_done_2_op (ds_abs1:ds_abs1_state) =
+ds_abs1 with <|
+state := if ds_abs1.ds_abs1_tx.tx_cur_length < ((LENGTH ds_abs1.ds_abs1_tx.tx_data_buffer) - 1)
+then abs1_tx_next else abs1_tx_last;
 ds_abs1_tx := ds_abs1.ds_abs1_tx with tx_cur_length := ds_abs1.ds_abs1_tx.tx_cur_length + 1 |>`
 
 (* comb_abs1_tx_reset_op: ds_abs1_state -> ds_abs1_state *)
@@ -70,6 +101,8 @@ val comb_abs1_tx_operations_def = Define `
 comb_abs1_tx_operations (ds_abs1:ds_abs1_state) =
 if ds_abs1.state = abs1_tx_trans 
 then (comb_abs1_tx_trans_op ds_abs1)
+else if ds_abs1.state = abs1_tx_done_2 
+then (comb_abs1_tx_done_2_op ds_abs1)
 else if ds_abs1.state = abs1_tx_reset 
 then (comb_abs1_tx_reset_op ds_abs1)
 else ds_abs1 with err := T`
@@ -80,7 +113,9 @@ else ds_abs1 with err := T`
 val ABS1_TX_LBL_ENABLE_def = Define `
 ABS1_TX_LBL_ENABLE (ds_abs1:ds_abs1_state) =
 ((ds_abs1.state = abs1_tx_done_1) \/
-(ds_abs1.state = abs1_tx_done_2))`
+(ds_abs1.state = abs1_tx_done_2) \/
+(ds_abs1.state = abs1_tx_next) \/
+(ds_abs1.state = abs1_tx_last))`
 
 (* abs1_tx_trans_done_op: ds_abs1_state -> ds_abs1_state * word8 option *)
 val abs1_tx_trans_done_op_def = Define `
@@ -90,6 +125,12 @@ if ds_abs1.state = abs1_tx_done_1 then
 SOME ds_abs1.spi_abs1.TX_SHIFT_REG)
 else if ds_abs1.state = abs1_tx_done_2 then
 (ds_abs1 with state := abs1_tx_trans,
+SOME ds_abs1.spi_abs1.TX_SHIFT_REG)
+else if ds_abs1.state = abs1_tx_next then
+(ds_abs1 with state := abs1_tx_update,
+SOME ds_abs1.spi_abs1.TX_SHIFT_REG)
+else if ds_abs1.state = abs1_tx_last then
+(ds_abs1 with state := abs1_tx_last_update,
 SOME ds_abs1.spi_abs1.TX_SHIFT_REG)
 else (ds_abs1 with err := T, NONE)`
 
