thm/abs1_comb_hold_ref_rel_WR_UPScript.sml
@@ -1,20 +1,644 @@
 open HolKernel bossLib boolLib Parse;
-open SPI_stateTheory SPI_relationTheory;
-open driver_stateTheory driver_relationTheory;
+open wordsLib pred_setLib;
+open SPI_stateTheory SPI_relationTheory SPI_update_regsTheory;
+open driver_stateTheory driver_relationTheory driver_writeTheory;
 open ds_abs1_stateTheory ds_abs1_relTheory ds_abs1_initTheory ds_abs1_txTheory 
 ds_abs1_rxTheory ds_abs1_xferTheory;
-open ref_relTheory;
+open ref_relTheory board_memTheory;
 
 val _ = new_theory "abs1_comb_hold_ref_rel_WR_UP";
 
 
-(* simulation: ds_abs1' exists and holds the ref_rel when driver_tau *)
+(* relation holds when driver state is dr_init_idle *)
+val ref_rel_hold_dr_init_idle_WR = store_thm("ref_rel_hold_dr_init_idle_WR",
+``!(spi:spi_state) (dr:driver_state) (ds_abs1:ds_abs1_state) (spi':spi_state).
+(ref_rel ds_abs1 dr spi) /\ (dr.state = dr_init_idle) /\
+(spi_tr spi (Update (THE (dr_write_address dr)) (THE (dr_write_value dr))) spi') ==>
+ref_rel ds_abs1 (dr_write_state dr) spi'``,
+rw [spi_tr_cases] >>
+rw [dr_write_state_def, dr_write_address_def, dr_write_value_def,
+dr_write_def, dr_write_softreset_def, write_SPI_regs_def] >|
+[FULL_SIMP_TAC (std_ss++PRED_SET_ss++WORD_ss) 
+[SPI0_SYSCONFIG_def, SPI0_PA_RANGE_def, SPI0_START_def, SPI0_END_def],
+`IS_STATE_REL ds_abs1 dr spi` by METIS_TAC [ref_rel_def] >>
+FULL_SIMP_TAC std_ss [IS_STATE_REL_def] >>
+rw [] >>
+Cases_on `dr.state` >>
+rw [] >>
+Cases_on `ds_abs1.state` >>
+rw [] >>
+Cases_on `spi.state` >>
+rw [] >>
+rw [write_SYSCONFIG_comb_def, write_SOFTRESET_def] >>
+FULL_SIMP_TAC std_ss [ref_rel_def, IS_STATE_REL_def] >>
+rw []]);
+
+
+(* relation holds for ds_abs1 or ds_abs1' when driver state is dr_init_setting *)
+val ref_rel_hold_dr_init_setting_WR = store_thm("ref_rel_hold_dr_init_setting_WR",
+``!(spi:spi_state) (dr:driver_state) (ds_abs1:ds_abs1_state) (spi':spi_state).
+(ref_rel ds_abs1 dr spi) /\ (dr.state = dr_init_setting) /\
+(spi_tr spi (Update (THE (dr_write_address dr)) (THE (dr_write_value dr))) spi') ==>
+(ref_rel ds_abs1 (dr_write_state dr) spi') \/
+(?ds_abs1'. (ds_abs1_tr ds_abs1 tau ds_abs1') /\ (ref_rel ds_abs1' (dr_write_state dr) spi'))``,
+rw [spi_tr_cases] >>
+rw [dr_write_state_def, dr_write_address_def, dr_write_value_def,dr_write_def] >|
+[ (* update SYSCONFIG *)
+rw [dr_write_sysconfig_def, write_SPI_regs_def, SPI0_SYSCONFIG_def, SPI0_PA_RANGE_def,
+SPI0_START_def, SPI0_END_def] >|
+[DISJ2_TAC >>
+`IS_STATE_REL ds_abs1 dr spi` by METIS_TAC [ref_rel_def] >>
+FULL_SIMP_TAC std_ss [IS_STATE_REL_def] >>
+rw [] >>
+Cases_on `dr.state` >>
+rw [] >>
+Cases_on `ds_abs1.state` >>
+rw [] >>
+Cases_on `spi.state` >>
+rw [] >>
+rw [ds_abs1_tr_cases, ds_abs1_comb_tr_cases] >>
+EXISTS_TAC ``comb_abs1_init_operations ds_abs1`` >>
+rw [COMB_ABS1_INIT_ENABLE_def, write_SYSCONFIG_comb_def, write_SYSCONFIG_def, 
+comb_abs1_init_operations_def, comb_abs1_init_start_op_def] >>
+FULL_SIMP_TAC std_ss [ref_rel_def, IS_STATE_REL_def] >>
+rw [] >>
+METIS_TAC [ref_rel_def],
+DISJ1_TAC >>
+rw [write_SYSCONFIG_comb_def, write_SYSCONFIG_def] >|
+[METIS_TAC [ref_rel_def],
+FULL_SIMP_TAC std_ss [ref_rel_def, IS_STATE_REL_def] >>
+rw [] >>
+METIS_TAC [],
+`IS_STATE_REL ds_abs1 dr spi` by METIS_TAC [ref_rel_def] >>
+FULL_SIMP_TAC std_ss [IS_STATE_REL_def] >>
+rw [] >>
+Cases_on `dr.state` >>
+rw [] >>
+Cases_on `ds_abs1.state` >>
+rw [] >>
+Cases_on `spi.state` >>
+rw []]],
+(* update MODULCTRL *)
+rw [dr_write_modulctrl_def, write_SPI_regs_def, SPI0_MODULCTRL_def, SPI0_SYSCONFIG_def, 
+SPI0_PA_RANGE_def, SPI0_START_def, SPI0_END_def] >|
+[DISJ2_TAC >>
+`IS_STATE_REL ds_abs1 dr spi` by METIS_TAC [ref_rel_def] >>
+FULL_SIMP_TAC std_ss [IS_STATE_REL_def] >>
+rw [] >>
+Cases_on `dr.state` >>
+rw [] >>
+Cases_on `ds_abs1.state` >>
+rw [] >>
+Cases_on `spi.state` >>
+rw [] >>
+rw [ds_abs1_tr_cases, ds_abs1_comb_tr_cases] >>
+EXISTS_TAC ``comb_abs1_init_operations ds_abs1`` >>
+rw [COMB_ABS1_INIT_ENABLE_def, write_MODULCTRL_def, comb_abs1_init_operations_def, 
+comb_abs1_init_start_op_def] >>
+FULL_SIMP_TAC std_ss [ref_rel_def, IS_STATE_REL_def] >>
+rw [] >>
+METIS_TAC [ref_rel_def],
+DISJ1_TAC >>
+rw [write_MODULCTRL_def] >|
+[METIS_TAC [ref_rel_def],
+FULL_SIMP_TAC std_ss [ref_rel_def, IS_STATE_REL_def] >>
+rw [] >>
+METIS_TAC [],
+`IS_STATE_REL ds_abs1 dr spi` by METIS_TAC [ref_rel_def] >>
+FULL_SIMP_TAC std_ss [IS_STATE_REL_def] >>
+rw [] >>
+Cases_on `dr.state` >>
+rw [] >>
+Cases_on `ds_abs1.state` >>
+rw [] >>
+Cases_on `spi.state` >>
+rw []]],
+(* update CH0CONF.WL *)
+rw [dr_write_ch0conf_wl_def, write_SPI_regs_def, SPI0_CH0CONF_def, SPI0_MODULCTRL_def, 
+SPI0_SYSCONFIG_def, SPI0_PA_RANGE_def, SPI0_START_def, SPI0_END_def] >|
+[DISJ2_TAC >>
+`IS_STATE_REL ds_abs1 dr spi` by METIS_TAC [ref_rel_def] >>
+FULL_SIMP_TAC std_ss [IS_STATE_REL_def] >>
+rw [] >>
+Cases_on `dr.state` >>
+rw [] >>
+Cases_on `ds_abs1.state` >>
+rw [] >>
+Cases_on `spi.state` >>
+rw [] >>
+rw [ds_abs1_tr_cases, ds_abs1_comb_tr_cases] >>
+EXISTS_TAC ``comb_abs1_init_operations ds_abs1`` >>
+rw [COMB_ABS1_INIT_ENABLE_def, write_CH0CONF_comb_def, write_CH0CONF_WL_def,
+comb_abs1_init_operations_def, comb_abs1_init_start_op_def] >|
+[FULL_SIMP_TAC std_ss [ref_rel_def, IS_STATE_REL_def] >>
+rw [],
+METIS_TAC [ref_rel_def],
+UNDISCH_TAC ``~(7w:word5 >+ 2w:word5)`` >>
+EVAL_TAC],
+DISJ1_TAC >>
+rw [write_CH0CONF_comb_def, write_CH0CONF_WL_def] >|
+[METIS_TAC [ref_rel_def],
+FULL_SIMP_TAC std_ss [ref_rel_def, IS_STATE_REL_def] >>
+rw [] >>
+METIS_TAC [],
+`IS_STATE_REL ds_abs1 dr spi` by METIS_TAC [ref_rel_def] >>
+FULL_SIMP_TAC std_ss [IS_STATE_REL_def] >>
+rw [] >>
+Cases_on `dr.state` >>
+rw [] >>
+Cases_on `ds_abs1.state` >>
+rw [] >>
+Cases_on `spi.state` >>
+rw [] >>
+UNDISCH_TAC ``~(7w:word5 >+ 2w:word5)`` >>
+EVAL_TAC]],
+(* update CH0CONF.IS,DPE,TRM etc bits *)
+rw [dr_write_ch0conf_mode_def, write_SPI_regs_def, SPI0_CH0CONF_def, SPI0_MODULCTRL_def, 
+SPI0_SYSCONFIG_def, SPI0_PA_RANGE_def, SPI0_START_def, SPI0_END_def] >|
+[DISJ2_TAC >>
+`IS_STATE_REL ds_abs1 dr spi` by METIS_TAC [ref_rel_def] >>
+FULL_SIMP_TAC std_ss [IS_STATE_REL_def] >>
+rw [] >>
+Cases_on `dr.state` >>
+rw [] >>
+Cases_on `ds_abs1.state` >>
+rw [] >>
+Cases_on `spi.state` >>
+rw [] >>
+rw [ds_abs1_tr_cases, ds_abs1_comb_tr_cases] >>
+EXISTS_TAC ``comb_abs1_init_operations ds_abs1`` >>
+rw [COMB_ABS1_INIT_ENABLE_def, write_CH0CONF_comb_def, write_CH0CONF_def,
+comb_abs1_init_operations_def, comb_abs1_init_start_op_def] >>
+FULL_SIMP_TAC std_ss [ref_rel_def, IS_STATE_REL_def] >>
+rw [] >>
+METIS_TAC [ref_rel_def],
+DISJ1_TAC >>
+rw [write_CH0CONF_comb_def, write_CH0CONF_def] >|
+[METIS_TAC [ref_rel_def],
+FULL_SIMP_TAC std_ss [ref_rel_def, IS_STATE_REL_def] >>
+rw [] >>
+METIS_TAC [],
+`IS_STATE_REL ds_abs1 dr spi` by METIS_TAC [ref_rel_def] >>
+FULL_SIMP_TAC std_ss [IS_STATE_REL_def] >>
+rw [] >>
+Cases_on `dr.state` >>
+rw [] >>
+Cases_on `ds_abs1.state` >>
+rw [] >>
+Cases_on `spi.state` >>
+rw []]],
+(* update CH0CONF.CLKD *)
+rw [dr_write_ch0conf_speed_def, write_SPI_regs_def, SPI0_CH0CONF_def, SPI0_MODULCTRL_def, 
+SPI0_SYSCONFIG_def, SPI0_PA_RANGE_def, SPI0_START_def, SPI0_END_def] >>
+DISJ2_TAC >>
+`IS_STATE_REL ds_abs1 dr spi` by METIS_TAC [ref_rel_def] >>
+FULL_SIMP_TAC std_ss [IS_STATE_REL_def] >>
+rw [] >>
+Cases_on `dr.state` >>
+rw [] >>
+Cases_on `ds_abs1.state` >>
+rw [] >>
+Cases_on `spi.state` >>
+rw [] >>
+rw [ds_abs1_tr_cases, ds_abs1_comb_tr_cases] >>
+EXISTS_TAC ``comb_abs1_init_operations ds_abs1`` >>
+rw [COMB_ABS1_INIT_ENABLE_def, write_CH0CONF_comb_def, write_CH0CONF_speed_def,
+comb_abs1_init_operations_def, comb_abs1_init_start_op_def] >>
+FULL_SIMP_TAC std_ss [ref_rel_def, IS_STATE_REL_def] >>
+rw [] >>
+METIS_TAC [ref_rel_def]]);
+
+
+(* relation holds when driver state is dr_tx_idle *)
+val ref_rel_hold_dr_tx_idle_WR = store_thm("ref_rel_hold_dr_tx_idle_WR",
+``!(spi:spi_state) (dr:driver_state) (ds_abs1:ds_abs1_state) (spi':spi_state).
+(ref_rel ds_abs1 dr spi) /\ (dr.state = dr_tx_idle) /\
+(spi_tr spi (Update (THE (dr_write_address dr)) (THE (dr_write_value dr))) spi') ==>
+ref_rel ds_abs1 (dr_write_state dr) spi'``,
+rw [spi_tr_cases] >>
+rw [dr_write_state_def, dr_write_address_def, dr_write_value_def,
+dr_write_def, dr_write_ch0conf_tx_def, write_SPI_regs_def] >>
+FULL_SIMP_TAC (std_ss++PRED_SET_ss++WORD_ss) 
+[SPI0_SYSCONFIG_def, SPI0_PA_RANGE_def, SPI0_START_def, SPI0_END_def, SPI0_CH0CONF_def,SPI0_MODULCTRL_def] >>
+`IS_STATE_REL ds_abs1 dr spi` by METIS_TAC [ref_rel_def] >>
+FULL_SIMP_TAC std_ss [IS_STATE_REL_def] >>
+rw [] >>
+Cases_on `dr.state` >>
+rw [] >>
+Cases_on `ds_abs1.state` >>
+rw [] >>
+Cases_on `spi.state` >>
+rw [] >>
+rw [write_CH0CONF_comb_def, write_CH0CONF_tx_def] >>
+FULL_SIMP_TAC std_ss [ref_rel_def, IS_STATE_REL_def] >>
+rw []);
+
+(* relation holds when driver state is dr_tx_conf_issued *)
+val ref_rel_hold_dr_tx_conf_issued_WR = store_thm("ref_rel_hold_dr_tx_conf_issued_WR",
+``!(spi:spi_state) (dr:driver_state) (ds_abs1:ds_abs1_state) (spi':spi_state).
+(ref_rel ds_abs1 dr spi) /\ (dr.state = dr_tx_conf_issued) /\
+(spi_tr spi (Update (THE (dr_write_address dr)) (THE (dr_write_value dr))) spi') ==>
+ref_rel ds_abs1 (dr_write_state dr) spi'``,
+rw [spi_tr_cases] >>
+rw [dr_write_state_def, dr_write_address_def, dr_write_value_def,
+dr_write_def, dr_write_ch0ctrl_def, write_SPI_regs_def] >>
+FULL_SIMP_TAC (std_ss++PRED_SET_ss++WORD_ss) 
+[SPI0_SYSCONFIG_def, SPI0_PA_RANGE_def, SPI0_START_def, SPI0_END_def, SPI0_CH0CONF_def,
+SPI0_MODULCTRL_def, SPI0_CH0CTRL_def] >>
+`IS_STATE_REL ds_abs1 dr spi` by METIS_TAC [ref_rel_def] >>
+FULL_SIMP_TAC std_ss [IS_STATE_REL_def] >>
+rw [] >>
+Cases_on `dr.state` >>
+rw [] >>
+Cases_on `ds_abs1.state` >>
+rw [] >>
+Cases_on `spi.state` >>
+rw [] >>
+rw [write_CH0CTRL_def] >>
+FULL_SIMP_TAC std_ss [ref_rel_def, IS_STATE_REL_def] >>
+rw []);
+
+(* ds_abs1' exists and ref_rel holds when driver state is dr_tx_write_data *)
+val ref_rel_hold_dr_tx_write_data_WR = store_thm("ref_rel_hold_dr_tx_write_data_WR",
+``!(spi:spi_state) (dr:driver_state) (ds_abs1:ds_abs1_state) (spi':spi_state).
+(ref_rel ds_abs1 dr spi) /\ (dr.state = dr_tx_write_data) /\
+(spi_tr spi (Update (THE (dr_write_address dr)) (THE (dr_write_value dr))) spi') ==>
+?ds_abs1'. (ds_abs1_tr ds_abs1 tau ds_abs1') /\
+(ref_rel ds_abs1' (dr_write_state dr) spi')``,
+rw [spi_tr_cases, ds_abs1_tr_cases, ds_abs1_comb_tr_cases] >>
+`IS_STATE_REL ds_abs1 dr spi` by METIS_TAC [ref_rel_def] >>
+FULL_SIMP_TAC std_ss [IS_STATE_REL_def] >>
+rw [] >>
+Cases_on `dr.state` >>
+rw [] >>
+Cases_on `ds_abs1.state` >>
+rw [] >>
+Cases_on `spi.state` >>
+rw [] >|
+[(* abs1_tx_trans *)
+EXISTS_TAC ``comb_abs1_tx_operations ds_abs1`` >>
+rw [COMB_ABS1_TX_ENABLE_def] >>
+rw [comb_abs1_tx_operations_def, comb_abs1_tx_trans_op_def] >|
+[`dr.dr_tx.tx_cur_length < (LENGTH dr.dr_tx.tx_data_buf) - 1` by METIS_TAC[ref_rel_def] >>
+rw [dr_write_state_def, dr_write_address_def, dr_write_value_def, dr_write_def, 
+dr_write_tx0_def, write_SPI_regs_def] >>
+FULL_SIMP_TAC (std_ss++PRED_SET_ss++WORD_ss) 
+[SPI0_SYSCONFIG_def, SPI0_PA_RANGE_def, SPI0_START_def, SPI0_END_def, 
+SPI0_CH0CONF_def,SPI0_MODULCTRL_def, SPI0_CH0CTRL_def, SPI0_TX0_def] >>
+rw [write_TX0_def] >>
+FULL_SIMP_TAC std_ss [ref_rel_def, IS_STATE_REL_def, CHECK_TXS_BIT_def] >>
+rw [] >>
+SIMP_TAC (std_ss++WORD_BIT_EQ_ss) [],
+`~ (dr.dr_tx.tx_cur_length < (LENGTH dr.dr_tx.tx_data_buf) - 1)` by METIS_TAC[ref_rel_def] >>
+rw [dr_write_state_def, dr_write_address_def, dr_write_value_def, dr_write_def, 
+dr_write_tx0_def, write_SPI_regs_def] >>
+FULL_SIMP_TAC (std_ss++PRED_SET_ss++WORD_ss) 
+[SPI0_SYSCONFIG_def, SPI0_PA_RANGE_def, SPI0_START_def, SPI0_END_def, 
+SPI0_CH0CONF_def,SPI0_MODULCTRL_def, SPI0_CH0CTRL_def, SPI0_TX0_def] >>
+rw [write_TX0_def] >>
+FULL_SIMP_TAC std_ss [ref_rel_def, IS_STATE_REL_def, CHECK_TXS_BIT_def] >>
+rw [] >>
+SIMP_TAC (std_ss++WORD_BIT_EQ_ss) []],
+(* abs1_tx_done_2 *)
+EXISTS_TAC ``comb_abs1_tx_operations ds_abs1`` >>
+rw [COMB_ABS1_TX_ENABLE_def] >>
+rw [comb_abs1_tx_operations_def, comb_abs1_tx_done_2_op_def] >|
+[`dr.dr_tx.tx_cur_length < (LENGTH dr.dr_tx.tx_data_buf) - 1` by METIS_TAC[ref_rel_def] >>
+rw [dr_write_state_def, dr_write_address_def, dr_write_value_def, dr_write_def, 
+dr_write_tx0_def, write_SPI_regs_def] >>
+FULL_SIMP_TAC (std_ss++PRED_SET_ss++WORD_ss) 
+[SPI0_SYSCONFIG_def, SPI0_PA_RANGE_def, SPI0_START_def, SPI0_END_def, 
+SPI0_CH0CONF_def,SPI0_MODULCTRL_def, SPI0_CH0CTRL_def, SPI0_TX0_def] >>
+rw [write_TX0_def] >>
+FULL_SIMP_TAC std_ss [ref_rel_def, IS_STATE_REL_def, CHECK_TXS_BIT_def] >>
+rw [] >>
+SIMP_TAC (std_ss++WORD_BIT_EQ_ss) [],
+`~ (dr.dr_tx.tx_cur_length < (LENGTH dr.dr_tx.tx_data_buf) - 1)` by METIS_TAC[ref_rel_def] >>
+rw [dr_write_state_def, dr_write_address_def, dr_write_value_def, dr_write_def, 
+dr_write_tx0_def, write_SPI_regs_def] >>
+FULL_SIMP_TAC (std_ss++PRED_SET_ss++WORD_ss) 
+[SPI0_SYSCONFIG_def, SPI0_PA_RANGE_def, SPI0_START_def, SPI0_END_def, 
+SPI0_CH0CONF_def,SPI0_MODULCTRL_def, SPI0_CH0CTRL_def, SPI0_TX0_def] >>
+rw [write_TX0_def] >>
+FULL_SIMP_TAC std_ss [ref_rel_def, IS_STATE_REL_def, CHECK_TXS_BIT_def] >>
+rw [] >>
+SIMP_TAC (std_ss++WORD_BIT_EQ_ss) []]]);
+
+(* relation holds when driver state is dr_tx_issue_disable *)
+val ref_rel_hold_dr_tx_issue_disable_WR = store_thm("ref_rel_hold_dr_tx_issue_disable_WR",
+``!(spi:spi_state) (dr:driver_state) (ds_abs1:ds_abs1_state) (spi':spi_state).
+(ref_rel ds_abs1 dr spi) /\ (dr.state = dr_tx_issue_disable) /\
+(spi_tr spi (Update (THE (dr_write_address dr)) (THE (dr_write_value dr))) spi') ==>
+ref_rel ds_abs1 (dr_write_state dr) spi'``,
+rw [spi_tr_cases] >>
+rw [dr_write_state_def, dr_write_address_def, dr_write_value_def,
+dr_write_def, dr_write_ch0ctrl_def, write_SPI_regs_def] >>
+FULL_SIMP_TAC (std_ss++PRED_SET_ss++WORD_ss) 
+[SPI0_SYSCONFIG_def, SPI0_PA_RANGE_def, SPI0_START_def, SPI0_END_def, 
+SPI0_CH0CONF_def,SPI0_MODULCTRL_def, SPI0_CH0CTRL_def] >>
+`IS_STATE_REL ds_abs1 dr spi` by METIS_TAC [ref_rel_def] >>
+FULL_SIMP_TAC std_ss [IS_STATE_REL_def] >>
+rw [] >>
+Cases_on `dr.state` >>
+rw [] >>
+Cases_on `ds_abs1.state` >>
+rw [] >>
+Cases_on `spi.state` >>
+rw [] >>
+rw [write_CH0CTRL_def] >>
+FULL_SIMP_TAC std_ss [ref_rel_def, IS_STATE_REL_def] >>
+rw []);
+
+(* ds_abs1' exists and ref_rel holds when driver state is dr_tx_reset_conf *)
+val ref_rel_hold_dr_tx_reset_conf_WR = store_thm("ref_rel_hold_dr_tx_reset_conf_WR",
+``!(spi:spi_state) (dr:driver_state) (ds_abs1:ds_abs1_state) (spi':spi_state).
+(ref_rel ds_abs1 dr spi) /\ (dr.state = dr_tx_reset_conf) /\
+(spi_tr spi (Update (THE (dr_write_address dr)) (THE (dr_write_value dr))) spi') ==>
+?ds_abs1'. (ds_abs1_tr ds_abs1 tau ds_abs1') /\
+(ref_rel ds_abs1' (dr_write_state dr) spi')``,
+rw [spi_tr_cases, ds_abs1_tr_cases, ds_abs1_comb_tr_cases] >>
+`IS_STATE_REL ds_abs1 dr spi` by METIS_TAC [ref_rel_def] >>
+FULL_SIMP_TAC std_ss [IS_STATE_REL_def] >>
+rw [] >>
+Cases_on `dr.state` >>
+rw [] >>
+Cases_on `ds_abs1.state` >>
+rw [] >>
+Cases_on `spi.state` >>
+rw [] >>
+EXISTS_TAC ``comb_abs1_tx_operations ds_abs1`` >>
+rw [COMB_ABS1_TX_ENABLE_def] >>
+rw [comb_abs1_tx_operations_def, comb_abs1_tx_reset_op_def, dr_write_state_def, 
+dr_write_value_def,dr_write_address_def, dr_write_def, dr_write_ch0conf_tx_def, 
+write_SPI_regs_def] >>
+FULL_SIMP_TAC (std_ss++PRED_SET_ss++WORD_ss) 
+[SPI0_SYSCONFIG_def, SPI0_PA_RANGE_def, SPI0_START_def, SPI0_END_def, SPI0_CH0CONF_def,
+SPI0_MODULCTRL_def] >>
+rw [write_CH0CONF_comb_def, write_CH0CONF_tx_def] >>
+FULL_SIMP_TAC std_ss [ref_rel_def, IS_STATE_REL_def] >>
+rw []);
+
+(* relation holds when driver state is dr_rx_idle *)
+val ref_rel_hold_dr_rx_idle_WR = store_thm("ref_rel_hold_dr_rx_idle_WR",
+``!(spi:spi_state) (dr:driver_state) (ds_abs1:ds_abs1_state) (spi':spi_state).
+(ref_rel ds_abs1 dr spi) /\ (dr.state = dr_rx_idle) /\
+(spi_tr spi (Update (THE (dr_write_address dr)) (THE (dr_write_value dr))) spi') ==>
+ref_rel ds_abs1 (dr_write_state dr) spi'``,
+rw [spi_tr_cases] >>
+rw [dr_write_state_def, dr_write_address_def, dr_write_value_def,
+dr_write_def, dr_write_ch0conf_rx_def, write_SPI_regs_def] >>
+FULL_SIMP_TAC (std_ss++PRED_SET_ss++WORD_ss) 
+[SPI0_SYSCONFIG_def, SPI0_PA_RANGE_def, SPI0_START_def, SPI0_END_def, SPI0_CH0CONF_def,
+SPI0_MODULCTRL_def] >>
+`IS_STATE_REL ds_abs1 dr spi` by METIS_TAC [ref_rel_def] >>
+FULL_SIMP_TAC std_ss [IS_STATE_REL_def] >>
+rw [] >>
+Cases_on `dr.state` >>
+rw [] >>
+Cases_on `ds_abs1.state` >>
+rw [] >>
+Cases_on `spi.state` >>
+rw [] >>
+rw [write_CH0CONF_comb_def, write_CH0CONF_rx_def] >>
+FULL_SIMP_TAC std_ss [ref_rel_def, IS_STATE_REL_def] >>
+rw []);
+
+(* relation holds when driver state is dr_rx_conf_issued *)
+val ref_rel_hold_dr_rx_conf_issued_WR = store_thm("ref_rel_hold_dr_rx_conf_issued_WR",
+``!(spi:spi_state) (dr:driver_state) (ds_abs1:ds_abs1_state) (spi':spi_state).
+(ref_rel ds_abs1 dr spi) /\ (dr.state = dr_rx_conf_issued) /\
+(spi_tr spi (Update (THE (dr_write_address dr)) (THE (dr_write_value dr))) spi') ==>
+ref_rel ds_abs1 (dr_write_state dr) spi'``,
+rw [spi_tr_cases] >>
+rw [dr_write_state_def, dr_write_address_def, dr_write_value_def,
+dr_write_def, dr_write_ch0ctrl_def, write_SPI_regs_def] >>
+FULL_SIMP_TAC (std_ss++PRED_SET_ss++WORD_ss) 
+[SPI0_SYSCONFIG_def, SPI0_PA_RANGE_def, SPI0_START_def, SPI0_END_def, SPI0_CH0CONF_def,
+SPI0_MODULCTRL_def, SPI0_CH0CTRL_def] >>
+`IS_STATE_REL ds_abs1 dr spi` by METIS_TAC [ref_rel_def] >>
+FULL_SIMP_TAC std_ss [IS_STATE_REL_def] >>
+rw [] >>
+Cases_on `dr.state` >>
+rw [] >>
+Cases_on `ds_abs1.state` >>
+rw [] >>
+Cases_on `spi.state` >>
+rw [] >>
+rw [write_CH0CTRL_def] >>
+FULL_SIMP_TAC std_ss [ref_rel_def, IS_STATE_REL_def] >>
+rw []);
+
+(* relation holds when driver state is dr_rx_issue_disable *)
+val ref_rel_hold_dr_rx_issue_disable_WR = store_thm("ref_rel_hold_dr_rx_issue_disable_WR",
+``!(spi:spi_state) (dr:driver_state) (ds_abs1:ds_abs1_state) (spi':spi_state).
+(ref_rel ds_abs1 dr spi) /\ (dr.state = dr_rx_issue_disable) /\
+(spi_tr spi (Update (THE (dr_write_address dr)) (THE (dr_write_value dr))) spi') ==>
+ref_rel ds_abs1 (dr_write_state dr) spi'``,
+rw [spi_tr_cases] >>
+rw [dr_write_state_def, dr_write_address_def, dr_write_value_def,
+dr_write_def, dr_write_ch0ctrl_def, write_SPI_regs_def] >>
+FULL_SIMP_TAC (std_ss++PRED_SET_ss++WORD_ss) 
+[SPI0_SYSCONFIG_def, SPI0_PA_RANGE_def, SPI0_START_def, SPI0_END_def, SPI0_CH0CONF_def,
+SPI0_MODULCTRL_def, SPI0_CH0CTRL_def] >>
+`IS_STATE_REL ds_abs1 dr spi` by METIS_TAC [ref_rel_def] >>
+FULL_SIMP_TAC std_ss [IS_STATE_REL_def] >>
+rw [] >>
+Cases_on `dr.state` >>
+rw [] >>
+Cases_on `ds_abs1.state` >>
+rw [] >>
+Cases_on `spi.state` >>
+rw [] >>
+rw [write_CH0CTRL_def] >>
+FULL_SIMP_TAC std_ss [ref_rel_def, IS_STATE_REL_def] >>
+rw []); 
+
+(* ds_abs1' exists and ref_rel holds when driver state is dr_rx_reset_conf *)
+val ref_rel_hold_dr_rx_reset_conf_WR = store_thm("ref_rel_hold_dr_rx_reset_conf_WR",
+``!(spi:spi_state) (dr:driver_state) (ds_abs1:ds_abs1_state) (spi':spi_state).
+(ref_rel ds_abs1 dr spi) /\ (dr.state = dr_rx_reset_conf) /\
+(spi_tr spi (Update (THE (dr_write_address dr)) (THE (dr_write_value dr))) spi') ==>
+?ds_abs1'. (ds_abs1_tr ds_abs1 tau ds_abs1') /\
+(ref_rel ds_abs1' (dr_write_state dr) spi')``,
+rw [spi_tr_cases, ds_abs1_tr_cases, ds_abs1_comb_tr_cases] >>
+`IS_STATE_REL ds_abs1 dr spi` by METIS_TAC [ref_rel_def] >>
+FULL_SIMP_TAC std_ss [IS_STATE_REL_def] >>
+rw [] >>
+Cases_on `dr.state` >>
+rw [] >>
+Cases_on `ds_abs1.state` >>
+rw [] >>
+Cases_on `spi.state` >>
+rw [] >>
+EXISTS_TAC ``comb_abs1_rx_operations ds_abs1`` >>
+rw [COMB_ABS1_RX_ENABLE_def] >>
+rw [comb_abs1_rx_operations_def, comb_abs1_rx_reset_op_def, dr_write_state_def, 
+dr_write_value_def,dr_write_address_def, dr_write_def, dr_write_ch0conf_rx_def, 
+write_SPI_regs_def] >>
+FULL_SIMP_TAC (std_ss++PRED_SET_ss++WORD_ss) 
+[SPI0_SYSCONFIG_def, SPI0_PA_RANGE_def, SPI0_START_def, SPI0_END_def, SPI0_CH0CONF_def,
+SPI0_MODULCTRL_def] >>
+rw [write_CH0CONF_comb_def, write_CH0CONF_rx_def] >>
+FULL_SIMP_TAC std_ss [ref_rel_def, IS_STATE_REL_def] >>
+rw []);
+
+(* relation holds when driver state is dr_xfer_idle *)
+val ref_rel_hold_dr_xfer_idle_WR = store_thm("ref_rel_hold_dr_xfer_idle_WR",
+``!(spi:spi_state) (dr:driver_state) (ds_abs1:ds_abs1_state) (spi':spi_state).
+(ref_rel ds_abs1 dr spi) /\ (dr.state = dr_xfer_idle) /\
+(spi_tr spi (Update (THE (dr_write_address dr)) (THE (dr_write_value dr))) spi') ==>
+ref_rel ds_abs1 (dr_write_state dr) spi'``,
+rw [spi_tr_cases] >>
+rw [dr_write_state_def, dr_write_address_def, dr_write_value_def,
+dr_write_def, dr_write_ch0conf_xfer_def, write_SPI_regs_def] >>
+FULL_SIMP_TAC (std_ss++PRED_SET_ss++WORD_ss) 
+[SPI0_SYSCONFIG_def, SPI0_PA_RANGE_def, SPI0_START_def, SPI0_END_def, SPI0_CH0CONF_def,
+SPI0_MODULCTRL_def] >>
+`IS_STATE_REL ds_abs1 dr spi` by METIS_TAC [ref_rel_def] >>
+FULL_SIMP_TAC std_ss [IS_STATE_REL_def] >>
+rw [] >>
+Cases_on `dr.state` >>
+rw [] >>
+Cases_on `ds_abs1.state` >>
+rw [] >>
+Cases_on `spi.state` >>
+rw [] >>
+rw [write_CH0CONF_comb_def, write_CH0CONF_xfer_def] >>
+FULL_SIMP_TAC std_ss [ref_rel_def, IS_STATE_REL_def] >>
+rw []);
+
+(* relation holds when driver state is dr_xfer_conf_issued *)
+val ref_rel_hold_dr_xfer_conf_issued_WR = store_thm("ref_rel_hold_dr_xfer_conf_issued_WR",
+``!(spi:spi_state) (dr:driver_state) (ds_abs1:ds_abs1_state) (spi':spi_state).
+(ref_rel ds_abs1 dr spi) /\ (dr.state = dr_xfer_conf_issued) /\
+(spi_tr spi (Update (THE (dr_write_address dr)) (THE (dr_write_value dr))) spi') ==>
+ref_rel ds_abs1 (dr_write_state dr) spi'``,
+rw [spi_tr_cases] >>
+rw [dr_write_state_def, dr_write_address_def, dr_write_value_def,
+dr_write_def, dr_write_ch0ctrl_def, write_SPI_regs_def] >>
+FULL_SIMP_TAC (std_ss++PRED_SET_ss++WORD_ss) 
+[SPI0_SYSCONFIG_def, SPI0_PA_RANGE_def, SPI0_START_def, SPI0_END_def, SPI0_CH0CONF_def,
+SPI0_MODULCTRL_def, SPI0_CH0CTRL_def] >>
+`IS_STATE_REL ds_abs1 dr spi` by METIS_TAC [ref_rel_def] >>
+FULL_SIMP_TAC std_ss [IS_STATE_REL_def] >>
+rw [] >>
+Cases_on `dr.state` >>
+rw [] >>
+Cases_on `ds_abs1.state` >>
+rw [] >>
+Cases_on `spi.state` >>
+rw [] >>
+rw [write_CH0CTRL_def] >>
+FULL_SIMP_TAC std_ss [ref_rel_def, IS_STATE_REL_def] >>
+rw []);
+
+(* ds_abs1' exists and ref_rel holds when driver state is dr_xfer_write_dataO *)
+val ref_rel_hold_dr_xfer_write_dataO_WR = store_thm("ref_rel_hold_dr_xfer_write_dataO_WR",
+``!(spi:spi_state) (dr:driver_state) (ds_abs1:ds_abs1_state) (spi':spi_state).
+(ref_rel ds_abs1 dr spi) /\ (dr.state = dr_xfer_write_dataO) /\
+(spi_tr spi (Update (THE (dr_write_address dr)) (THE (dr_write_value dr))) spi') ==>
+?ds_abs1'. (ds_abs1_tr ds_abs1 tau ds_abs1') /\
+(ref_rel ds_abs1' (dr_write_state dr) spi')``,
+rw [spi_tr_cases, ds_abs1_tr_cases, ds_abs1_comb_tr_cases] >>
+`IS_STATE_REL ds_abs1 dr spi` by METIS_TAC [ref_rel_def] >>
+FULL_SIMP_TAC std_ss [IS_STATE_REL_def] >>
+rw [] >>
+Cases_on `dr.state` >>
+rw [] >>
+Cases_on `ds_abs1.state` >>
+rw [] >>
+Cases_on `spi.state` >>
+rw [] >>
+EXISTS_TAC ``comb_abs1_xfer_operations ds_abs1`` >>
+rw [COMB_ABS1_XFER_ENABLE_def] >>
+rw [comb_abs1_xfer_operations_def, comb_abs1_xfer_prepare_op_def,
+dr_write_state_def, dr_write_address_def, dr_write_value_def, dr_write_def,
+dr_write_tx0_def, write_SPI_regs_def] >>
+FULL_SIMP_TAC (std_ss++PRED_SET_ss++WORD_ss) 
+[SPI0_SYSCONFIG_def, SPI0_PA_RANGE_def, SPI0_START_def, SPI0_END_def, 
+SPI0_CH0CONF_def,SPI0_MODULCTRL_def, SPI0_CH0CTRL_def, SPI0_TX0_def] >>
+rw [write_TX0_def] >>
+FULL_SIMP_TAC std_ss [ref_rel_def, IS_STATE_REL_def, CHECK_TXS_BIT_def] >>
+rw [] >>
+SIMP_TAC (std_ss++WORD_BIT_EQ_ss) []);
+
+(* relation holds when driver state is dr_xfer_issue_disable *)
+val ref_rel_hold_dr_xfer_issue_disable_WR = store_thm("ref_rel_hold_dr_xfer_issue_disable_WR",
+``!(spi:spi_state) (dr:driver_state) (ds_abs1:ds_abs1_state) (spi':spi_state).
+(ref_rel ds_abs1 dr spi) /\ (dr.state = dr_xfer_issue_disable) /\
+(spi_tr spi (Update (THE (dr_write_address dr)) (THE (dr_write_value dr))) spi') ==>
+ref_rel ds_abs1 (dr_write_state dr) spi'``,
+rw [spi_tr_cases] >>
+rw [dr_write_state_def, dr_write_address_def, dr_write_value_def,
+dr_write_def, dr_write_ch0ctrl_def, write_SPI_regs_def] >>
+FULL_SIMP_TAC (std_ss++PRED_SET_ss++WORD_ss) 
+[SPI0_SYSCONFIG_def, SPI0_PA_RANGE_def, SPI0_START_def, SPI0_END_def, SPI0_CH0CONF_def,
+SPI0_MODULCTRL_def, SPI0_CH0CTRL_def] >>
+`IS_STATE_REL ds_abs1 dr spi` by METIS_TAC [ref_rel_def] >>
+FULL_SIMP_TAC std_ss [IS_STATE_REL_def] >>
+rw [] >>
+Cases_on `dr.state` >>
+rw [] >>
+Cases_on `ds_abs1.state` >>
+rw [] >>
+Cases_on `spi.state` >>
+rw [] >>
+rw [write_CH0CTRL_def] >>
+FULL_SIMP_TAC std_ss [ref_rel_def, IS_STATE_REL_def] >>
+rw []);
+
+(* ds_abs1' exists and ref_rel holds when driver state is dr_xfer_reset_conf *)
+val ref_rel_hold_dr_xfer_reset_conf_WR = store_thm("ref_rel_hold_dr_xfer_reset_conf_WR",
+``!(spi:spi_state) (dr:driver_state) (ds_abs1:ds_abs1_state) (spi':spi_state).
+(ref_rel ds_abs1 dr spi) /\ (dr.state = dr_xfer_reset_conf) /\
+(spi_tr spi (Update (THE (dr_write_address dr)) (THE (dr_write_value dr))) spi') ==>
+?ds_abs1'. (ds_abs1_tr ds_abs1 tau ds_abs1') /\
+(ref_rel ds_abs1' (dr_write_state dr) spi')``,
+rw [spi_tr_cases, ds_abs1_tr_cases, ds_abs1_comb_tr_cases] >>
+`IS_STATE_REL ds_abs1 dr spi` by METIS_TAC [ref_rel_def] >>
+FULL_SIMP_TAC std_ss [IS_STATE_REL_def] >>
+rw [] >>
+Cases_on `dr.state` >>
+rw [] >>
+Cases_on `ds_abs1.state` >>
+rw [] >>
+Cases_on `spi.state` >>
+rw [] >>
+EXISTS_TAC ``comb_abs1_xfer_operations ds_abs1`` >>
+rw [COMB_ABS1_XFER_ENABLE_def] >>
+rw [comb_abs1_xfer_operations_def, comb_abs1_xfer_reset_op_def, dr_write_state_def, 
+dr_write_value_def,dr_write_address_def, dr_write_def, dr_write_ch0conf_xfer_def, 
+write_SPI_regs_def] >>
+FULL_SIMP_TAC (std_ss++PRED_SET_ss++WORD_ss) 
+[SPI0_SYSCONFIG_def, SPI0_PA_RANGE_def, SPI0_START_def, SPI0_END_def, SPI0_CH0CONF_def,SPI0_MODULCTRL_def] >>
+rw [write_CH0CONF_comb_def, write_CH0CONF_xfer_def] >>
+FULL_SIMP_TAC std_ss [ref_rel_def, IS_STATE_REL_def] >>
+rw []);
+
+(* simulation: ref_rel holds for ds_abs1 or ds_abs1' when driver and controller perform WRITE and UPDATE operations *)
 val abs1_comb_hold_ref_rel_WR_UP = store_thm("abs1_comb_hold_ref_rel_WR_UP",
-``!(spi:spi_state) (dr:driver_state) (ds_abs1:ds_abs1_state).
+``!(spi:spi_state) (dr:driver_state) (ds_abs1:ds_abs1_state) (a:word32) (v:word32) 
+(spi':spi_state) (dr':driver_state).
 (ref_rel ds_abs1 dr spi) /\ (driver_tr dr (Write a v) dr') /\ 
 (spi_tr spi (Update a v) spi') ==>
 (ref_rel ds_abs1 dr' spi') \/
 (?ds_abs1'. (ds_abs1_tr ds_abs1 tau ds_abs1') /\ (ref_rel ds_abs1' dr' spi'))``,
-cheat);
+rw [driver_tr_cases, DR_WR_ENABLE_def] >|
+[METIS_TAC [ref_rel_hold_dr_init_idle_WR],
+METIS_TAC [ref_rel_hold_dr_init_setting_WR],
+METIS_TAC [ref_rel_hold_dr_tx_idle_WR],
+METIS_TAC [ref_rel_hold_dr_tx_conf_issued_WR],
+METIS_TAC [ref_rel_hold_dr_tx_write_data_WR],
+METIS_TAC [ref_rel_hold_dr_tx_issue_disable_WR],
+METIS_TAC [ref_rel_hold_dr_tx_reset_conf_WR],
+METIS_TAC [ref_rel_hold_dr_rx_idle_WR],
+METIS_TAC [ref_rel_hold_dr_rx_conf_issued_WR],
+METIS_TAC [ref_rel_hold_dr_rx_issue_disable_WR],
+METIS_TAC [ref_rel_hold_dr_rx_reset_conf_WR],
+METIS_TAC [ref_rel_hold_dr_xfer_idle_WR],
+METIS_TAC [ref_rel_hold_dr_xfer_conf_issued_WR],
+METIS_TAC [ref_rel_hold_dr_xfer_write_dataO_WR],
+METIS_TAC [ref_rel_hold_dr_xfer_issue_disable_WR],
+METIS_TAC [ref_rel_hold_dr_xfer_reset_conf_WR]]);
 
 val _ = export_theory();
