thm/abs1_comb_hold_ref_rel_dr_trScript.sml
@@ -50,35 +50,66 @@ val ref_rel_check_tx_eot = store_thm("ref_rel_check_tx_eot",
 (ref_rel ds_abs1 dr spi) /\ (dr.dr_last_read_ad = SOME SPI0_CH0STAT) /\
 (dr.dr_last_read_v = SOME v) /\ (dr.state = dr_tx_check_eot) ==>
 (ref_rel ds_abs1 (dr_check_tx_ch0stat dr v) spi)``,
-rw [dr_check_tx_ch0stat_def] >|
-[FULL_SIMP_TAC std_ss [ref_rel_def, IS_STATE_REL_def] >>
+rw [dr_check_tx_ch0stat_def] >>
+FULL_SIMP_TAC std_ss [ref_rel_def, IS_STATE_REL_def] >>
 rw [] >>
 Cases_on `spi.state` >>
-rw [] >> 
-FULL_SIMP_TAC (std_ss++WORD_ss) [],
-FULL_SIMP_TAC std_ss [ref_rel_def, IS_STATE_REL_def] >>
-rw [],
-Cases_on `(2 >< 2) v: word1` >>
-FULL_SIMP_TAC (arith_ss ++ WORD_ss) [] >>
-Cases_on `n` >>
-FULL_SIMP_TAC (arith_ss++WORD_ss) [] >>
-Cases_on `n'` >>
-FULL_SIMP_TAC (arith_ss++WORD_ss) []]);
+rw []);
 
 (* driver tau transition to check RXS Bit for rx automaton *)
 val ref_rel_check_rx_rxs = store_thm("ref_rel_check_rx_rxs",
 ``!(spi:spi_state) (dr:driver_state) (ds_abs1:ds_abs1_state) (v:word32).
 (ref_rel ds_abs1 dr spi) /\ (dr.dr_last_read_ad = SOME SPI0_CH0STAT) /\
 (dr.dr_last_read_v = SOME v) /\ (dr.state = dr_rx_check_rxs) ==>
-(ref_rel ds_abs1 (dr_check_rx_ch0stat dr v) spi)``,
+(ref_rel ds_abs1 (dr_check_rx_ch0stat dr v) spi) \/
+(?ds_abs1'. (ds_abs1_tr ds_abs1 tau ds_abs1') /\ 
+(ref_rel ds_abs1' (dr_check_rx_ch0stat dr v) spi))``,
 rw [dr_check_rx_ch0stat_def] >|
-[FULL_SIMP_TAC std_ss [ref_rel_def, IS_STATE_REL_def] >>
+[(* RXS = 1w /\ left_length > 0 *)
+`IS_STATE_REL ds_abs1 dr spi` by METIS_TAC [ref_rel_def] >>
+FULL_SIMP_TAC std_ss [IS_STATE_REL_def] >>
+rw [] >>
+Cases_on `dr.state` >>
+rw [] >>
+Cases_on `ds_abs1.state` >>
 rw [] >>
 Cases_on `spi.state` >>
-rw [] >> 
-FULL_SIMP_TAC (std_ss++WORD_ss) [],
+rw [] >|
+[FULL_SIMP_TAC (std_ss++WORD_ss) [ref_rel_def],
+FULL_SIMP_TAC (std_ss++WORD_ss) [ref_rel_def],
+FULL_SIMP_TAC (std_ss++WORD_ss) [ref_rel_def],
+DISJ2_TAC >>
+`ds_abs1.ds_abs1_rx.rx_left_length > 0` by METIS_TAC [ref_rel_def] >>
+rw [ds_abs1_tr_cases, ds_abs1_dr_tr_cases, DRIVER_ABS1_RX_ENABLE_def] >>
+EXISTS_TAC ``driver_abs1_rx_operations ds_abs1`` >>
+rw [driver_abs1_rx_operations_def, driver_abs1_rx_ready_op_def] >>
+FULL_SIMP_TAC std_ss [ref_rel_def, IS_STATE_REL_def] >>
+rw []],
+(* RXS = 1w /\ left_length < 0 *)
+`~ (dr.dr_rx.rx_left_length > 0)` by FULL_SIMP_TAC std_ss [] >>
+`IS_STATE_REL ds_abs1 dr spi` by METIS_TAC [ref_rel_def] >>
+FULL_SIMP_TAC std_ss [IS_STATE_REL_def] >>
+rw [] >>
+Cases_on `dr.state` >>
+rw [] >>
+Cases_on `ds_abs1.state` >>
+rw [] >>
+Cases_on `spi.state` >>
+rw [] >|
+[FULL_SIMP_TAC (std_ss++WORD_ss) [ref_rel_def],
+FULL_SIMP_TAC (std_ss++WORD_ss) [ref_rel_def],
+FULL_SIMP_TAC (std_ss++WORD_ss) [ref_rel_def],
+DISJ2_TAC >>
+`~(ds_abs1.ds_abs1_rx.rx_left_length > 0)` by METIS_TAC [ref_rel_def] >>
+rw [ds_abs1_tr_cases, ds_abs1_dr_tr_cases, DRIVER_ABS1_RX_ENABLE_def] >>
+EXISTS_TAC ``driver_abs1_rx_operations ds_abs1`` >>
+rw [driver_abs1_rx_operations_def, driver_abs1_rx_ready_op_def] >>
+FULL_SIMP_TAC std_ss [ref_rel_def, IS_STATE_REL_def] >>
+rw []],
+(* RXS = 0w *)
 FULL_SIMP_TAC std_ss [ref_rel_def, IS_STATE_REL_def] >>
 rw []]);
+
 
 (* lemma:dr.state = dr_rx_fetch_data -> 
    ds_abs1 is able to perform tau_driver operations, according to ref_rel *)
@@ -140,39 +171,25 @@ EXISTS_TAC ``driver_abs1_rx_operations ds_abs1`` >>
 `DRIVER_ABS1_RX_ENABLE ds_abs1` by METIS_TAC [dr_rx_fetch_data_imply_driver_abs1_rx_enable] >>
 FULL_SIMP_TAC std_ss [DRIVER_ABS1_RX_ENABLE_def] >>
 rw [dr_check_rx0_def, driver_abs1_rx_operations_def] >|
-[(* abs1_rx_fetch_data, left_length > 1 *)
-`ds_abs1.ds_abs1_rx.rx_left_length > 1` by METIS_TAC [ref_rel_def] >>
+[(* abs1_rx_ready, illegal state *)
+FULL_SIMP_TAC std_ss [ref_rel_def, IS_STATE_REL_def] >>
+rw [],
+(* abs1_rx_fetch_data *)
 rw [driver_abs1_rx_fetch_data_op_def] >>
 FULL_SIMP_TAC (std_ss++WORD_ss) [ref_rel_def, IS_STATE_REL_def] >>
 rw [],
-(* abs1_rx_fetch_data, left_length = 1 *)
-`~ (ds_abs1.ds_abs1_rx.rx_left_length > 1)` by METIS_TAC [ref_rel_def] >>
-rw [driver_abs1_rx_fetch_data_op_def] >>
-FULL_SIMP_TAC (std_ss++WORD_ss) [ref_rel_def, IS_STATE_REL_def] >>
-rw [],
-(* abs1_rx_next, left_length > 1 *)
-`ds_abs1.ds_abs1_rx.rx_left_length > 1` by METIS_TAC [ref_rel_def] >>
+(* abs1_rx_next *)
 rw [driver_abs1_rx_next_op_def] >>
 FULL_SIMP_TAC (std_ss++WORD_ss) [ref_rel_def, IS_STATE_REL_def] >>
 rw [],
-(* abs1_rx_next, left_length = 1 *)
-`~ (ds_abs1.ds_abs1_rx.rx_left_length > 1)` by METIS_TAC [ref_rel_def] >>
-rw [driver_abs1_rx_next_op_def] >>
-FULL_SIMP_TAC (std_ss++WORD_ss) [ref_rel_def, IS_STATE_REL_def] >>
-rw [],
-(* abs1_rx_next_ready, left_length > 1 *)
-`ds_abs1.ds_abs1_rx.rx_left_length > 1` by METIS_TAC [ref_rel_def] >>
-rw [driver_abs1_rx_next_ready_op_def] >>
-FULL_SIMP_TAC (std_ss++WORD_ss) [ref_rel_def, IS_STATE_REL_def] >>
-rw [],
-`~ (ds_abs1.ds_abs1_rx.rx_left_length > 1)` by METIS_TAC [ref_rel_def] >>
+(* abs1_rx_next_ready *)
 rw [driver_abs1_rx_next_ready_op_def] >>
 FULL_SIMP_TAC (std_ss++WORD_ss) [ref_rel_def, IS_STATE_REL_def] >>
 rw []]);
 
 
 val ref_rel_check_xfer_txs = store_thm("ref_rel_check_xfer_txs",
-``!(spi:spi_state) (dr:driver_state) (ds_abs1:ds_abs1_state).
+``!(spi:spi_state) (dr:driver_state) (ds_abs1:ds_abs1_state) (v:word32).
 (ref_rel ds_abs1 dr spi) /\ (dr.dr_last_read_ad = SOME SPI0_CH0STAT) /\
 (dr.dr_last_read_v = SOME v) /\ (dr.state = dr_xfer_check_txs) ==>
 (ref_rel ds_abs1 (dr_check_xfer_ch0stat dr v) spi)``,
@@ -192,7 +209,7 @@ Cases_on `n'` >>
 FULL_SIMP_TAC (arith_ss++WORD_ss) []]);
 
 val ref_rel_check_xfer_rxs = store_thm("ref_rel_check_xfer_rxs",
-``!(spi:spi_state) (dr:driver_state) (ds_abs1:ds_abs1_state).
+``!(spi:spi_state) (dr:driver_state) (ds_abs1:ds_abs1_state) (v:word32).
 (ref_rel ds_abs1 dr spi) /\ (dr.dr_last_read_ad = SOME SPI0_CH0STAT) /\
 (dr.dr_last_read_v = SOME v) /\ (dr.state = dr_xfer_check_rxs) ==>
 (ref_rel ds_abs1 (dr_check_xfer_ch0stat dr v) spi)``,
@@ -258,7 +275,7 @@ Cases_on `ds_abs1.state` >>
 rw []);
 
 val ref_rel_check_xfer_rx0 = store_thm("ref_rel_check_xfer_rx0",
-``!(spi:spi_state) (dr:driver_state) (ds_abs1:ds_abs1_state).
+``!(spi:spi_state) (dr:driver_state) (ds_abs1:ds_abs1_state) (v:word32).
 (ref_rel ds_abs1 dr spi) /\ (dr.dr_last_read_ad = SOME SPI0_RX0) /\
 (dr.dr_last_read_v = SOME v) /\ (dr.state = dr_xfer_fetch_dataI) ==>
 ?ds_abs1'. (ds_abs1_tr ds_abs1 tau ds_abs1') /\ 
@@ -281,7 +298,7 @@ rw []]);
 
 (* simulation: ds_abs1' exists and holds the ref_rel when driver_tau *)
 val abs1_comb_hold_ref_rel_driver_tr = store_thm("abs1_comb_hold_ref_rel_driver_tr",
-``!(spi:spi_state) (dr:driver_state) (ds_abs1:ds_abs1_state).
+``!(spi:spi_state) (dr:driver_state) (ds_abs1:ds_abs1_state) (dr':driver_state).
 (ref_rel ds_abs1 dr spi) /\ (driver_tr dr tau dr') ==>
 (ref_rel ds_abs1 dr' spi) \/
 (?ds_abs1'. (ds_abs1_tr ds_abs1 tau ds_abs1') /\ (ref_rel ds_abs1' dr' spi))``,
