thm/ref_rel_holds_trans_lblScript.sml
@@ -8,58 +8,48 @@ open ref_relTheory;
 val _ = new_theory "ref_rel_holds_trans_lbl";
 
 (* a lemma to determine ds_abs1.state *)
-(* If spi.state = tx_trans_done, then ds_abs1 is also able to perform TX label transition *)
+(* If spi.state = tx_trans_done or tx_trans_next, then ds_abs1 is also able to perform TX label transition *)
 val spi_tx_trans_done_imply_abs1_tx_enable = store_thm("spi_tx_trans_done_imply_abs1_tx_enable",
 ``!(spi:spi_state) (dr:driver_state) (ds_abs1:ds_abs1_state).
-(ref_rel ds_abs1 dr spi) /\ (spi.state = tx_trans_done) ==>
+(ref_rel ds_abs1 dr spi) /\ 
+(spi.state = tx_trans_done \/ spi.state = tx_trans_next) ==>
 (ABS1_TX_LBL_ENABLE ds_abs1)``,
 rw [ABS1_TX_LBL_ENABLE_def] >>
 `IS_STATE_REL ds_abs1 dr spi` by METIS_TAC[ref_rel_def] >>
 FULL_SIMP_TAC std_ss [IS_STATE_REL_def] >>
 Cases_on `dr.state` >>
 rw [] >>
-`(spi.state <> init_start) /\
-(spi.state <> init_reset) /\
-(spi.state <> init_setregs) /\
-(spi.state <> spi_ready) /\
-(spi.state <> tx_conf_ready) /\
-(spi.state <> tx_channel_enabled) /\
-(spi.state <> tx_ready_for_trans) /\
-(spi.state <> tx_trans_data) /\
-(spi.state <> tx_channel_disabled) /\
-(spi.state <> rx_conf_ready) /\
-(spi.state <> rx_channel_enabled) /\
-(spi.state <> rx_receive_data) /\
-(spi.state <> rx_update_RX0) /\
-(spi.state <> rx_data_ready) /\
-(spi.state <> rx_channel_disabled) /\
-(spi.state <> xfer_conf_ready) /\
-(spi.state <> xfer_channel_enabled) /\
-(spi.state <> xfer_ready_for_trans) /\
-(spi.state <> xfer_trans_data) /\
-(spi.state <> xfer_exchange_data) /\
-(spi.state <> xfer_update_RX0) /\
-(spi.state <> xfer_data_ready) /\
-(spi.state <> xfer_channel_disabled)` by rw [] >>
 Cases_on `ds_abs1.state` >>
+rw [] >>
+Cases_on `spi.state` >>
 rw []);
 
 (* bisimulation: ds_abs1' exists for TX label *)
 val abs1_comb_hold_ref_rel_TX = store_thm("abs1_comb_hold_ref_rel_TX",
-``!(spi:spi_state) (dr:driver_state) (ds_abs1:ds_abs1_state) (data:word8 option).
+``!(spi:spi_state) (dr:driver_state) (ds_abs1:ds_abs1_state) (data:word8 option) (spi':spi_state).
 (ref_rel ds_abs1 dr spi) /\ (spi_tr spi (TX data) spi') ==>
 ?ds_abs1'. (ds_abs1_tr ds_abs1 (TX data) ds_abs1') /\ (ref_rel ds_abs1' dr spi')``,
 rw [spi_tr_cases] >>
 `ABS1_TX_LBL_ENABLE ds_abs1` by METIS_TAC[spi_tx_trans_done_imply_abs1_tx_enable] >>
 rw [ds_abs1_tr_cases] >|
-[(* output data equals *)
-rw [tx_trans_done_op_value_def, tx_trans_done_op_def, 
+[(* output data equals when spi.state = tx_trans_done *)
+rw [tx_TX_op_value_def, tx_TX_op_def, tx_trans_done_op_def,
 abs1_tx_trans_done_op_value_def, abs1_tx_trans_done_op_def] >>
 METIS_TAC[ref_rel_def, ABS1_TX_LBL_ENABLE_def],
-(* ref_rel holds *)
+(* ref_rel holds when spi.state = tx_trans_done *)
 FULL_SIMP_TAC std_ss [ABS1_TX_LBL_ENABLE_def] >>
 rw [abs1_tx_trans_done_op_state_def, abs1_tx_trans_done_op_def,
-tx_trans_done_op_state_def, tx_trans_done_op_def] >>
+tx_TX_op_state_def, tx_TX_op_def, tx_trans_done_op_def] >>
+FULL_SIMP_TAC std_ss [ref_rel_def, IS_STATE_REL_def] >>
+rw [],
+(* output data equals when spi.state = tx_trans_next *)
+rw [tx_TX_op_value_def, tx_TX_op_def, tx_trans_next_op_def,
+abs1_tx_trans_done_op_value_def, abs1_tx_trans_done_op_def] >>
+METIS_TAC[ref_rel_def, ABS1_TX_LBL_ENABLE_def],
+(* ref_rel holds when spi.state = tx_trans_next *)
+FULL_SIMP_TAC std_ss [ABS1_TX_LBL_ENABLE_def] >>
+rw [abs1_tx_trans_done_op_state_def, abs1_tx_trans_done_op_def,
+tx_TX_op_state_def, tx_TX_op_def, tx_trans_next_op_def] >>
 FULL_SIMP_TAC std_ss [ref_rel_def, IS_STATE_REL_def] >>
 rw []]);
 
@@ -70,16 +60,37 @@ val comb_abs1_hold_ref_rel_TX = store_thm("comb_abs1_hold_ref_rel_TX",
 ?dr' spi'. (local_tr (dr, spi) (TX (abs1_tx_trans_done_op_value ds_abs1)) (dr', spi')) /\
 (ref_rel (abs1_tx_trans_done_op_state ds_abs1) dr' spi')``,
 rw [local_tr_cases, spi_tr_cases] >|
-[`spi.state = tx_trans_done` by METIS_TAC[ABS1_TX_LBL_ENABLE_def, ref_rel_def, IS_STATE_REL_def] >>
+[`spi.state = tx_trans_done \/ spi.state = tx_trans_next` 
+by METIS_TAC[ABS1_TX_LBL_ENABLE_def, ref_rel_def, IS_STATE_REL_def] >>
 rw [abs1_tx_trans_done_op_value_def, abs1_tx_trans_done_op_def, 
-tx_trans_done_op_value_def, tx_trans_done_op_def] >>
+tx_TX_op_value_def, tx_TX_op_def, tx_trans_done_op_def, tx_trans_next_op_def] >>
 FULL_SIMP_TAC std_ss [ref_rel_def, ABS1_TX_LBL_ENABLE_def],
 METIS_TAC [ABS1_TX_LBL_ENABLE_def, ref_rel_def, IS_STATE_REL_def],
-`spi.state = tx_trans_done` by METIS_TAC[ABS1_TX_LBL_ENABLE_def, ref_rel_def, IS_STATE_REL_def] >>
+FULL_SIMP_TAC std_ss [ABS1_TX_LBL_ENABLE_def] >|
+[(* abs1_tx_done_1 *)
+`spi.state = tx_trans_done` by METIS_TAC[ref_rel_def, IS_STATE_REL_def] >>
 rw [abs1_tx_trans_done_op_state_def, abs1_tx_trans_done_op_def,
-tx_trans_done_op_state_def, tx_trans_done_op_def] >>
-FULL_SIMP_TAC std_ss [ref_rel_def, ABS1_TX_LBL_ENABLE_def, IS_STATE_REL_def] >>
-rw []]);
+tx_TX_op_state_def, tx_TX_op_def, tx_trans_done_op_def] >>
+FULL_SIMP_TAC std_ss [ref_rel_def, IS_STATE_REL_def] >>
+rw [],
+(* abs1_tx_done_2 *)
+`spi.state = tx_trans_done` by METIS_TAC[ref_rel_def, IS_STATE_REL_def] >>
+rw [abs1_tx_trans_done_op_state_def, abs1_tx_trans_done_op_def,
+tx_TX_op_state_def, tx_TX_op_def, tx_trans_done_op_def] >>
+FULL_SIMP_TAC std_ss [ref_rel_def, IS_STATE_REL_def] >>
+rw [],
+(* abs1_tx_next *)
+`spi.state = tx_trans_next` by METIS_TAC[ref_rel_def, IS_STATE_REL_def] >>
+rw [abs1_tx_trans_done_op_state_def, abs1_tx_trans_done_op_def,
+tx_TX_op_state_def, tx_TX_op_def, tx_trans_next_op_def] >>
+FULL_SIMP_TAC std_ss [ref_rel_def, IS_STATE_REL_def] >>
+rw [],
+(* abs1_tx_last *)
+`spi.state = tx_trans_next` by METIS_TAC[ref_rel_def, IS_STATE_REL_def] >>
+rw [abs1_tx_trans_done_op_state_def, abs1_tx_trans_done_op_def,
+tx_TX_op_state_def, tx_TX_op_def, tx_trans_next_op_def] >>
+FULL_SIMP_TAC std_ss [ref_rel_def, IS_STATE_REL_def] >>
+rw []]]);
 
 (* a lemma for RX label proof *)
 (* If spi.state = rx_receive_data, then abs1 is able to process RX label as well. *)
@@ -92,36 +103,15 @@ rw [ABS1_RX_LBL_ENABLE_def] >>
 FULL_SIMP_TAC std_ss [IS_STATE_REL_def] >>
 Cases_on `dr.state` >>
 rw [] >>
-`(spi.state <> init_start) /\
-(spi.state <> init_reset) /\
-(spi.state <> init_setregs) /\
-(spi.state <> spi_ready) /\
-(spi.state <> tx_conf_ready) /\
-(spi.state <> tx_channel_enabled) /\
-(spi.state <> tx_ready_for_trans) /\
-(spi.state <> tx_trans_data) /\
-(spi.state <> tx_trans_done) /\
-(spi.state <> tx_channel_disabled) /\
-(spi.state <> rx_conf_ready) /\
-(spi.state <> rx_channel_enabled) /\
-(spi.state <> rx_update_RX0) /\
-(spi.state <> rx_data_ready) /\
-(spi.state <> rx_channel_disabled) /\
-(spi.state <> xfer_conf_ready) /\
-(spi.state <> xfer_channel_enabled) /\
-(spi.state <> xfer_ready_for_trans) /\
-(spi.state <> xfer_trans_data) /\
-(spi.state <> xfer_exchange_data) /\
-(spi.state <> xfer_update_RX0) /\
-(spi.state <> xfer_data_ready) /\
-(spi.state <> xfer_channel_disabled)` by rw [] >>
 Cases_on `ds_abs1.state` >>
+rw [] >>
+Cases_on `spi.state` >>
 rw []);
 
 
 (* bisimulation: ds_abs1' exists for RX label *)
 val abs1_comb_hold_ref_rel_RX = store_thm("abs1_comb_hold_ref_rel_RX",
-``!(spi:spi_state) (dr:driver_state) (ds_abs1:ds_abs1_state) (data:word8 option).
+``!(spi:spi_state) (dr:driver_state) (ds_abs1:ds_abs1_state) (data:word8 option) (spi':spi_state).
 (ref_rel ds_abs1 dr spi) /\ (spi_tr spi (RX data) spi') ==>
 ?ds_abs1'. (ds_abs1_tr ds_abs1 (RX data) ds_abs1') /\ (ref_rel ds_abs1' dr spi')``,
 rw [spi_tr_cases, ds_abs1_tr_cases] >|
@@ -129,7 +119,7 @@ rw [spi_tr_cases, ds_abs1_tr_cases] >|
 `ABS1_RX_LBL_ENABLE ds_abs1` by METIS_TAC [spi_rx_receive_data_imply_abs1_rx_enable] >>
 FULL_SIMP_TAC std_ss [ABS1_RX_LBL_ENABLE_def] >>
 rw [abs1_rx_receive_data_op_def, rx_receive_data_op_def, abs1_rx_receive_op_def,
-abs1_rx_fetch_data_op_def, abs1_rx_done_op_def] >>
+abs1_rx_fetch_data_op_def] >>
 FULL_SIMP_TAC (std_ss++WORD_ss) [ref_rel_def, IS_STATE_REL_def] >>
 rw []]);
 
@@ -145,7 +135,7 @@ rw [local_tr_cases, spi_tr_cases] >|
 `spi.state = rx_receive_data` by METIS_TAC[ref_rel_def, IS_STATE_REL_def, ABS1_RX_LBL_ENABLE_def] >>
 FULL_SIMP_TAC std_ss [ABS1_RX_LBL_ENABLE_def] >>
 rw [abs1_rx_receive_data_op_def, abs1_rx_receive_op_def,
-abs1_rx_fetch_data_op_def, abs1_rx_done_op_def, rx_receive_data_op_def] >>
+abs1_rx_fetch_data_op_def, rx_receive_data_op_def] >>
 FULL_SIMP_TAC std_ss [ref_rel_def, IS_STATE_REL_def] >>
 rw []]);
 
@@ -160,35 +150,14 @@ rw [] >>
 FULL_SIMP_TAC std_ss [IS_STATE_REL_def] >>
 Cases_on `dr.state` >>
 rw [] >>
-`(spi.state <> init_start) /\
-(spi.state <> init_reset) /\
-(spi.state <> init_setregs) /\
-(spi.state <> spi_ready) /\
-(spi.state <> tx_conf_ready) /\
-(spi.state <> tx_channel_enabled) /\
-(spi.state <> tx_ready_for_trans) /\
-(spi.state <> tx_trans_data) /\
-(spi.state <> tx_trans_done) /\
-(spi.state <> tx_channel_disabled) /\
-(spi.state <> rx_conf_ready) /\
-(spi.state <> rx_channel_enabled) /\
-(spi.state <> rx_receive_data) /\
-(spi.state <> rx_update_RX0) /\
-(spi.state <> rx_data_ready) /\
-(spi.state <> rx_channel_disabled) /\
-(spi.state <> xfer_conf_ready) /\
-(spi.state <> xfer_channel_enabled) /\
-(spi.state <> xfer_ready_for_trans) /\
-(spi.state <> xfer_trans_data) /\ 
-(spi.state <> xfer_update_RX0) /\
-(spi.state <> xfer_data_ready) /\
-(spi.state <> xfer_channel_disabled)` by rw [] >>
 Cases_on `ds_abs1.state` >>
+rw [] >>
+Cases_on `spi.state` >>
 rw []);
 
 (* bisimulation: ds_abs1' holds for XFER label *)
 val abs1_comb_hold_ref_rel_XFER = store_thm("abs1_comb_hold_ref_rel_XFER",
-``!(spi:spi_state) (dr:driver_state) (ds_abs1:ds_abs1_state) (dataIN:word8 option) (dataOUT:word8 option).
+``!(spi:spi_state) (dr:driver_state) (ds_abs1:ds_abs1_state) (dataIN:word8 option) (dataOUT:word8 option) (spi':spi_state).
 (ref_rel ds_abs1 dr spi) /\ (spi_tr spi (XFER dataIN dataOUT) spi') ==>
 ?ds_abs1'. (ds_abs1_tr ds_abs1 (XFER dataIN dataOUT) ds_abs1') /\ (ref_rel ds_abs1' dr spi')``,
 rw [spi_tr_cases] >>
